update

HolBA/src/tools/parallelcomposition/deduction/interleavingdeductionScript.sml
@@ -83,10 +83,6 @@ Inductive binterl:
   (((binterl (t1:('event1 + 'eventS) option list) (t2:('event2 + 'eventS) option list) t) /\ (t1' = (SOME (INL e1)::t1)) /\ (t' = (SOME (INL (INL e1))::t))) ==> (binterl t1' t2 t')) /\
 [~right:]                                                                        
   (((binterl (t1:('event1 + 'eventS) option list) (t2:('event2 + 'eventS) option list) t) /\ (t2' = (SOME (INL e2)::t2)) /\ (t' = (SOME (INR (INL e2))::t))) ==> (binterl t1 t2' t')) /\
-[~leftN:]
-  (((binterl (t1:('event1 + 'eventS) option list) (t2:('event2 + 'eventS) option list) t) /\ (t1' = (SOME (INL e1)::t1)) /\ (t2' = (NONE::t2)) /\ (t' = (SOME (INL (INL e1))::t))) ==> (binterl t1' t2' t')) /\
-[~rightN:]                                                                        
-  (((binterl (t1:('event1 + 'eventS) option list) (t2:('event2 + 'eventS) option list) t) /\ (t1' = (NONE::t1)) /\ (t2' = (SOME (INL e2)::t2)) /\ (t' = (SOME (INR (INL e2))::t))) ==> (binterl t1' t2' t')) /\
 [~syncR:]                                                                        
   (((binterl (t1:('event1 + 'eventS) option list) (t2:('event2 + 'eventS) option list) t) /\ (t1' = (SOME (INR e)::t1)) /\ (t2' = (SOME (INR e)::t2)) /\ (t' = (SOME (INR (INR e))::t))) ==> (binterl t1' t2' t')) /\
 [~syncL:]                                                                        
@@ -102,23 +98,12 @@ Inductive binterl:
 [~movenone:]                                                                        
   ((binterl (NONE::(t1:('event1 + 'eventS) option list)) (NONE::(t2:('event2 + 'eventS) option list)) (NONE::t)) ==> (binterl t1 t2 t))  /\
 [~movecombinenone:]                                                                        
-  ((binterl (t1:('event1 + 'eventS) option list) (t2:('event2 + 'eventS) option list) (NONE::t)) ==> (binterl t1 t2 t)) /\
-[~moveB:]
-  (((binterl ((h1::t1):('event1 + 'eventS) option list) ((h2::t2):('event2 + 'eventS) option list) (h::t))∧(binterl [h1] [h2] [h])) ==> (binterl t1 t2 t))/\
-[~moveF:]
-  (((binterl t1 t2 t) ∧ (binterl [h1] [h2] [h])) ==> (binterl ((h1::t1):('event1 + 'eventS) option list) ((h2::t2):('event2 + 'eventS) option list) (h::t))) /\
-[~single:]
-  (((binterl t1 t2 t) ∧ (binterl ((h1::t1):('event1 + 'eventS) option list) ((h2::t2):('event2 + 'eventS) option list) (h::t))) ==> (binterl [h1] [h2] [h]))
+  ((binterl (t1:('event1 + 'eventS) option list) (t2:('event2 + 'eventS) option list) (NONE::t)) ==> (binterl t1 t2 t)) 
 End
 
 val binterl_Empty = new_axiom ("binterl_Empty",
                                ``∀t1 t2. binterl t1 t2 [] ⇒ ((t1 = []) ∧(t2 = []))``);
 
-val binterl_Conj = new_axiom ("binterl_Conj",
-                              ``∀h1 t1 h2 t2 h t. (binterl ((h1::t1):('event1 + 'eventS) option list) ((h2::t2):('event2 + 'eventS) option list) (h::t)) ⇒ ((binterl t1 t2 t) ∧ (binterl [h1] [h2] [h]))``);
-
-val binterl_NotEmpty = new_axiom ("binterl_NotEmpty",
-                                  ``∀t1 t2. binterl t1 t2 (h::t) ⇒ (∃h1 t1' h2 t2'. (t1 = (h1::t1'))∧(t2 = (h2::t2')))``);
                                
 val binterl_moveSL = new_axiom ("binterl_moveNONE",
                                 ``∀e t t1 t2.
@@ -134,16 +119,6 @@ val binterl_moveSR = new_axiom ("binterl_moveSR",
                                      binterl t1 t2 (SOME (INR (INR e))::t) ⇒
                                    (∃t1' t2'. (t1 = SOME (INR e)::t1') ∧(t2 = SOME (INR e)::t2'))``);
 
- val binterl_moveNAL = new_axiom ("binterl_moveNAL",
-                               ``∀e1 t t1 t2.
-                                     binterl t1 t2 (SOME (INL (INL e1))::t) ⇒
-                                  (∃t1' t2'. (t1 = SOME (INL e1)::t1') ∧ (t2 = NONE::t2'))``);
-
-val binterl_moveNAR = new_axiom ("binterl_moveNAR",
-                                 ``∀e2 t t1 t2.
-                                       binterl t1 t2 (SOME (INR (INL e2))::t) ⇒
-                                    (∃t1' t2'. (t2 = SOME (INL e2)::t2') ∧ (t1 = NONE::t1'))``);
-
  val binterl_moveAL = new_axiom ("binterl_moveAL",
                                ``∀e1 t t1 t2.
                                      binterl t1 t2 (SOME (INL (INL e1))::t) ⇒
@@ -153,25 +128,7 @@ val binterl_moveAR = new_axiom ("binterl_moveAR",
                                      binterl t1 t2 (SOME (INR (INL e2))::t) ⇒
                                   (∃t2'. (t2 = SOME (INL e2)::t2'))``);                                  
 
-val binterl_moveALN = new_axiom ("binterl_moveALN",
-                               ``∀e1.
-                                     binterl [SOME (INL e1)] [NONE] [SOME (INL (INL e1))] =
-                                  (binterl [] [] [])``);
-
-val binterl_moveSLN = new_axiom ("binterl_moveSLN",
-                               ``∀e2.
-                                     binterl [NONE] [SOME (INR e2)] [SOME (INL (INR e2))] =
-                                  (binterl [] [] [])``);
-
-val binterl_moveSRN = new_axiom ("binterl_moveSRN",
-                                 ``∀e2.                                  
-                                      binterl [NONE] [SOME (INR e2)] [SOME (INR (INR e2))] =
-                                    (binterl [] [] [])``);
-
-val binterl_moveARN = new_axiom ("binterl_moveARN",
-                               ``∀e2.
-binterl [NONE] [SOME (INL e2)] [SOME (INR (INL e2))] =
-                                  (binterl [] [] [])``);  
+ 
 
 Definition binterleave_ts:
   binterleave_ts ts1 ts2 = {t| ∃t1 t2. (t1 ∈ ts1) ∧ (t2 ∈ ts2) ∧ (binterl t1 t2 t)}
