HolBA/src/tools/parallelcomposition/examples/XOR/Combination-XOR.sml
@@ -39,10 +39,13 @@ val prog_lbl_tms_ = get_block_dict_keys bl_dict_;
 
 val prog_vars = gen_vars_of_prog prog_tm;
 
-    
-val lbl_tm = ``BL_Address (Imm64 4203632w)``;
+val bv_key = ``BVar "key" (BType_Imm Bit64)``;
 
-val stop_lbl_tms = [``BL_Address (Imm64 4203756w)``]; 
+val prog_vars = bv_key::prog_vars;
+    
+val lbl_tm = ``BL_Address (Imm64 60w)``;
+
+val stop_lbl_tms = [``BL_Address (Imm64 132w)``]; 
 
 val n_dict = bir_cfgLib.cfg_build_node_dict bl_dict_ prog_lbl_tms_;
 
@@ -74,28 +77,45 @@ val _ = print "\n";
 val predlists = List.map (fn syst => ((rev o SYST_get_pred) syst))
                          systs_noassertfailed;
 
-val tr = predlist_to_tree predlists;
+val _ = print "Get predlists";
+val _ = print "\n";
+    
+val predlists_refined = List.map (fn lst => bir_symbexec_sortLib.removeDuplicates lst) predlists;
+val _ = print "Get refined predlists";    
+val _ = print "\n";
+(* val _ = printTermList predlists_refined; *)
+    
+val tree = predlist_to_tree predlists_refined;
 
+val _ = print "Get tree";
+val _ = print "\n";
+    
 val vals_list = bir_symbexec_treeLib.symb_execs_vals_term systs_noassertfailed [];
+
+val _ = print "Get vals_list";
+val _ = print "\n";
+	
 val sort_vals = bir_symbexec_sortLib.refine_symb_val_list vals_list;
 
+val _ = print "Get sort_vals";
+val _ = print "\n";    
 
-val valtr =  tree_with_value tr sort_vals;
-
-val _ = print "\n";     
+val valtr =  tree_with_value tree sort_vals;
+     
 val _ = print ("built a symbolic tree with value");
 val _ = print "\n";
 
 
-val sapic_process = sbir_tree_sapic_process (purge_tree valtr);
-
-
-val _ = print "\n";     
-val _ = print ("sapic_process");
-val _ = print "\n";
+val sapic_process = sbir_tree_sapic_process sort_vals (purge_tree valtr);
     
-val _ =  ( write_sapic_to_file o process_to_string) sapic_process
+val _ = print ("built sapic_process");
+val _ = print "\n";
 
-val _ = print "\n";     
+
+val refined_process = refine_process sapic_process;
+	
+val _ =  ( write_sapic_to_file o process_to_string) refined_process;
+     
 val _ = print ("wrote into file");
 val _ = print "\n";
+
