HolBA/src/tools/parallelcomposition/sapic/synceventsSyntax.sig
@@ -16,6 +16,11 @@ val mk_A2P : term -> term
 val Sync_Fr_tm : term
 val dest_Sync_Fr : term -> term
 val is_Sync_Fr : term -> bool
-val mk_Sync_Fr : term -> term			       
+val mk_Sync_Fr : term -> term
+val Crypto_tm : term
+val dest_Crypto : term -> term
+val is_Crypto : term -> bool
+val mk_Crypto :  term -> term
+			 
 
 end
