HolBA/src/tools/parallelcomposition/translateTosapic/translate_to_sapicLib.sml
@@ -267,6 +267,9 @@ fun bir_exp_to_sapic_term exp =
 	else if (identical exp “bir_exp_true”)
 	then
 		(mk_Con (mk_Name (PubName_tm, “"1"”)),(Thm.INST_TYPE [alpha |-> (type_of exp)] EQ_REFL))
+	else if (identical exp “bir_exp_false”)
+	then
+		(mk_Con (mk_Name (PubName_tm, “"0"”)),(Thm.INST_TYPE [alpha |-> (type_of exp)] EQ_REFL))
 	else
 	    let
 		val (name,trms) = strip_comb exp;
