HolBA/src/tools/parallelcomposition/tree/sbir_treeLib.sml
@@ -43,41 +43,59 @@ fun allHeadsEqual ([]: term list list) = false
 
 (* Define a datatype for trees *)
 datatype 'a tree = Leaf | Node of 'a * 'a tree | Branch of 'a * 'a tree * 'a tree;
-	 
+
+(* Helper function to check if all lists in a list are empty *)
+fun all_empty lsts = List.all null lsts
+
+(* Helper function to check if a list is not empty *)
+fun not_empty ls = not (null ls)
+
+fun prtion (lst: term list list) = case lst of
+				       ([]: term list list) => ([], [])
+				     | ([[]]: term list list) => ([], [])
+				     | ((h::_): term list list) => 
+				       let
+					   val head_val = ((hd h):term) 
+				       in
+					   List.partition (fn (ls: term list) => (identical (hd ls) head_val)) lst
+				       end
+				       
+(* Main function to convert predicate lists to tree *)
 fun predlist_to_tree ([[]]: term list list) = Leaf
   | predlist_to_tree ([]: term list list) = Leaf
-  | predlist_to_tree (lst: term list list) =    
-    if (is_true_list (List.map (fn ls => (null ls)) lst)) then Leaf
+  | predlist_to_tree (lsts: term list list) =    
+    if all_empty lsts then Leaf
     else
 	let
-	val (empty, notempty) =
-	    if ((exists is_false (List.map (fn ls => (null ls)) lst)) andalso (exists is_true (List.map (fn ls => (null ls)) lst)))
-	    then List.partition (fn ls => (null ls)) lst
-	    else ([[]],lst)
-		    
-	val (head_eq, head_noteq) = if ((not o null o hd) notempty)
-				    then List.partition (fn ls => (identical ((hd o hd) notempty) (hd ls))) notempty
-				    else List.partition (fn ls => (identical ((hd o hd o rev) notempty) (hd ls))) notempty;
-    in
-	    if (null head_noteq)
-	    then
-		    (Node ((hd (hd head_eq)), (predlist_to_tree (List.map (fn ls => (tl ls)) head_eq))))handle _ => raise ERR "predlist_to_tree" ("cannot do it "^(String.concat(List.map (fn ls => ("\n"^((int_to_string o List.length) ls))) head_eq)))
-	    else
-		if ((not o null) head_eq) then
-		    if ((not o null o hd) head_eq)
-		    then
-			Branch ((hd (hd head_eq)),(predlist_to_tree (List.map (fn ls => (tl ls)) head_eq)),(predlist_to_tree (List.map (fn ls => (tl ls)) head_noteq)))
-		    else predlist_to_tree head_noteq
-		else predlist_to_tree head_noteq
-		     
-    end
+           
+            val (empty, notempty) = List.partition null lsts
 
-	
+	    val (head_eq, head_noteq) = prtion notempty;
+	in    
+	    if null head_noteq then
+		Node (hd (hd head_eq), predlist_to_tree (List.map tl head_eq))
+	    else
+		
+		    Branch (
+		    
+		    hd (hd head_noteq),
+		  
+		    (predlist_to_tree (List.map (fn ls => (tl ls)) head_noteq))handle _ => raise ERR "predlist_to_tree" ("cannot do it "^(String.concat(List.map (fn ls => ("|n"^((int_to_string o List.length) ls))) head_eq))),
+		  
+		    (predlist_to_tree (List.map (fn ls => (tl ls)) head_eq))handle _ => raise ERR "predlist_to_tree" ("cannot do it "^(String.concat(List.map (fn ls => ("|n"^((int_to_string o List.length) ls))) head_noteq)))
+		    )
+	end 
+
+	 
+
+
 (*Find bir expression*)
 fun find_be_val vals_list bv =
     let
 	val find_val = List.find (fn (a,_) => Term.term_eq a bv) vals_list;
-	val symbv = ((snd o Option.valOf) find_val) handle _ => raise ERR "find_be_val" ("cannot find symbolic value for "^(term_to_string bv)^"\n");
+	val (bv_str, _) = bir_envSyntax.dest_BVar_string bv;
+	val fr = get_bvar_fresh (bir_envSyntax.mk_BVar_string (bv_str, “BType_Bool”)); 
+	val symbv = ((snd o Option.valOf) find_val) handle _ => SymbValBE (fr, Redblackset.empty Term.compare) ;
 	val exp =
 	    case symbv of
 		SymbValBE (x, _) => x
@@ -105,15 +123,66 @@ fun hd_of_tree tr =
       | VBranch ((bv,be), subtr1, subtr2) => SOME (bv,be)
 
 
+fun areIdentical bv x =
+    if (bir_expSyntax.is_BExp_Den x andalso bir_expSyntax.is_BExp_Den bv) orelse (bir_envSyntax.is_BVar x andalso bir_envSyntax.is_BVar bv) orelse (bir_envSyntax.is_bir_var_name x andalso bir_envSyntax.is_bir_var_name bv) then
+        identical x bv
+	 else if stringSyntax.is_string bv then
+        identical x (bir_envSyntax.mk_BVar (bv, “BType_Imm Bit64”))
+    else if stringSyntax.is_string x then
+        identical (bir_envSyntax.mk_BVar (x, “BType_Imm Bit64”)) bv
+    else
+        raise ERR "areIdentical " ((term_to_string bv) ^ " compare to " ^ (term_to_string x))
+
+	      
+fun trmunion(xs: term list, ys: term list) = foldl (fn (x, acc) => if List.exists (fn y => (identical x y)) acc then acc else x::acc) ys xs
+					     
+fun liveVars tr = 
+    case tr of
+	VLeaf => ((Redblackset.empty Term.compare): term Redblackset.set)
+      | VNode ((bv,be), subtr) =>
+	let
+            val subtrLive = ((liveVars subtr): term Redblackset.set);
+            val exprLive =  if (bir_envSyntax.is_BVar be)
+			    then [be]
+			    else ((bir_exp_helperLib.get_birexp_vars be)handle _ =>
+									       let
+										   val (name,trms) = strip_comb be;
+									       in
+										   trms
+									       end
+									       
+				 );
+	    val strLive = List.map (fn x => (fst o bir_envSyntax.dest_BVar) x) exprLive;
+	    val combinedLive = Redblackset.addList(subtrLive,strLive);
+        in
+            (combinedLive: term Redblackset.set)
+        end
+      | VBranch ((bv,be), subtr1, subtr2) =>
+	let
+            val leftLive = liveVars subtr1;
+            val rightLive = liveVars subtr2;
+	    val combinedLive = Redblackset.union(leftLive,rightLive);
+        in
+            (combinedLive: term Redblackset.set)
+        end
+	
+	
 fun purge_tree tr =
     case tr of
 	VLeaf => VLeaf
-      | VNode ((bv,be), subtr) => if (isSome (hd_of_tree subtr)) then
-				      if ((identical ((fst o valOf o hd_of_tree) subtr) bv) andalso (identical ((snd o valOf o hd_of_tree) subtr) be))
-				      then (purge_tree subtr)
-				      else VNode ((bv,be), (purge_tree subtr))
-				  else VNode ((bv,be), (purge_tree subtr))
-      | VBranch ((bv,be), subtr1, subtr2) => VBranch ((bv,be), (purge_tree subtr1), (purge_tree subtr2))					     
+      | VNode ((bv,be), subtr) =>
+	if (isSome (hd_of_tree subtr)) then
+	    if ((identical ((fst o valOf o hd_of_tree) subtr) bv) andalso (identical ((snd o valOf o hd_of_tree) subtr) be))
+	    then (purge_tree subtr)
+	    else VNode ((bv,be), (purge_tree subtr))
+	else VNode ((bv,be), (purge_tree subtr))
+      | VBranch ((bv,be), subtr1, subtr2) =>
+	if (identical be “BExp_Const (Imm1 1w)”)
+	then (purge_tree subtr1)
+	else if (identical be “BExp_Const (Imm1 0w)”)
+	then (purge_tree subtr2)
+	else VBranch ((bv,be), (purge_tree subtr1), (purge_tree subtr2))
+	     
 
 
 end (* local *)
