HolBA/src/tools/parallelcomposition/generaldeduction/interleavinggeneraldeductionScript.sml
@@ -22,6 +22,10 @@ Inductive binterl:
   (((binterl (t1:('event1 + 'eventS) option list) (t2:('event2 + 'eventS) option list) t) /\ (t1' = (SOME (INL e1)::t1)) /\ (t' = (SOME (INL (INL e1))::t))) ==> (binterl t1' t2 t')) /\
 [~right:]                                                                        
   (((binterl (t1:('event1 + 'eventS) option list) (t2:('event2 + 'eventS) option list) t) /\ (t2' = (SOME (INL e2)::t2)) /\ (t' = (SOME (INR (INL e2))::t))) ==> (binterl t1 t2' t')) /\
+[~leftN:]
+  (((binterl (t1:('event1 + 'eventS) option list) (t2:('event2 + 'eventS) option list) t) /\ (t1' = (SOME (INL e1)::t1)) /\ (t2' = (NONE::t2)) /\ (t' = (SOME (INL (INL e1))::t))) ==> (binterl t1' t2' t')) /\
+[~rightN:]                                                                        
+  (((binterl (t1:('event1 + 'eventS) option list) (t2:('event2 + 'eventS) option list) t) /\ (t1' = (NONE::t1)) /\ (t2' = (SOME (INL e2)::t2)) /\ (t' = (SOME (INR (INL e2))::t))) ==> (binterl t1' t2' t')) /\
 [~syncR:]                                                                        
   (((binterl (t1:('event1 + 'eventS) option list) (t2:('event2 + 'eventS) option list) t) /\ (t1' = (SOME (INR e)::t1)) /\ (t2' = (SOME (INR e)::t2)) /\ (t' = (SOME (INR (INR e))::t))) ==> (binterl t1' t2' t')) /\
 [~syncL:]                                                                        
@@ -41,7 +45,13 @@ Inductive binterl:
 [~movenone:]                                                                        
   ((binterl (NONE::(t1:('event1 + 'eventS) option list)) (NONE::(t2:('event2 + 'eventS) option list)) (NONE::t)) ==> (binterl t1 t2 t))  /\
 [~movecombinenone:]                                                                        
-  ((binterl (t1:('event1 + 'eventS) option list) (t2:('event2 + 'eventS) option list) (NONE::t)) ==> (binterl t1 t2 t)) 
+  ((binterl (t1:('event1 + 'eventS) option list) (t2:('event2 + 'eventS) option list) (NONE::t)) ==> (binterl t1 t2 t)) /\
+[~moveB:]
+  (((binterl ((h1::t1):('event1 + 'eventS) option list) ((h2::t2):('event2 + 'eventS) option list) (h::t))∧(binterl [h1] [h2] [h])) ==> (binterl t1 t2 t))/\
+[~moveF:]
+  (((binterl t1 t2 t) ∧ (binterl [h1] [h2] [h])) ==> (binterl ((h1::t1):('event1 + 'eventS) option list) ((h2::t2):('event2 + 'eventS) option list) (h::t))) /\
+[~single:]
+  (((binterl t1 t2 t) ∧ (binterl ((h1::t1):('event1 + 'eventS) option list) ((h2::t2):('event2 + 'eventS) option list) (h::t))) ==> (binterl [h1] [h2] [h]))
 End
 
 
@@ -49,12 +59,79 @@ Definition binterleave_ts:
   binterleave_ts ts1 ts2 = {t| ∃t1 t2. (t1 ∈ ts1) ∧ (t2 ∈ ts2) ∧ (binterl t1 t2 t)}
 End
 
+
+val doubleLeftMTrn_def =
+Define`
+      doubleLeftMTrn (MTrn:('event + 'eventS, 'pred, 'state, 'symb) mtrel) (v,(p: ('predL + 'pred) -> bool),(c:'stateL),s) (t:(('event + 'eventS)+('eventL + 'eventS)) option list) (v',(p': ('predL + 'pred) -> bool),(c':'stateL),s')  = (MTrn (v,(IMAGE OUTR p),s) (MAP (OPTION_MAP OUTL) t) (v',(IMAGE OUTR p'),s'))
+`;
+
+val doubleRightMTrn_def =
+Define`
+      doubleRightMTrn (MTrn:('event + 'eventS, 'pred, 'state, 'symb) mtrel) (v,(p: ('pred + 'predR) -> bool),s,(c:'stateR)) (t:(('event + 'eventS)+('eventR + 'eventS)) option list) (v',(p': ('pred + 'predR) -> bool),s',(c':'stateR))  = (MTrn (v,(IMAGE OUTL p),s) (MAP (OPTION_MAP OUTL) t) (v',(IMAGE OUTL p'),s'))
+`;
+
+
+val doubleLeftDed_def =
+Define `
+       (doubleLeftDed (ded: ('pred) tded) (p: ('predL + 'pred) -> bool) (phi: ('predL + 'pred))  =  (ded (IMAGE OUTR p) (OUTR phi))
+       )`;  
         
+val doubleRightDed_def =
+Define `
+       (doubleRightDed (ded: ('pred) tded) (p: ('pred + 'predR) -> bool) (phi: ('pred + 'predR))  =  (ded (IMAGE OUTL p) (OUTL phi))
+       )`;
+
+       
+val prSum_def =
+Define`
+      prSum (P :(('pred1 + 'pred2) + ('pred1 + 'pred2) + 'pred3) -> bool) (P' :('pred1 + 'pred2 + 'pred3) + 'pred2 + 'pred3) =
+(∀x. (x ∈ P) ∧
+(case x of
+  INL (INL (ll : 'pred1)) => (ll = (OUTL (OUTL P')))
+| INR (INR (rr: 'pred3)) => (rr = (OUTR (OUTR P')))
+| INL (INR (lr : 'pred2)) => (lr = (OUTL (OUTR (OUTL P'))))
+| INR (INL (INL (rll : 'pred1))) => (rll = (OUTL (OUTL P')))
+| INR (INL (INR (rlr : 'pred2))) => (rlr = (OUTL (OUTR P')))
+))
+`;
+
+
+val prSumRev_def =
+Define`
+      prSumRev (P :(('pred1 + 'pred2 + 'pred3) + 'pred2 + 'pred3) -> bool) (P' :('pred1 + 'pred2) + ('pred1 + 'pred2) + 'pred3)  =
+(∀x. (x ∈ P) ∧
+(case x of
+  INL (INL (ll : 'pred1)) => (ll = (OUTL (OUTL P'))) 
+| INR (INR (rr: 'pred3)) => (rr = (OUTR (OUTR P')))
+| INL (INR (INL (lrl : 'pred2))) => (lrl = (OUTR (OUTL (OUTR P'))))
+| INR (INL (rl : 'pred2)) => (rl = (OUTR (OUTL (OUTR P'))))
+| INL (INR (INR (lrr : 'pred3))) => (lrr = (OUTR (OUTR P'))) 
+))
+`;
+        
+val prSum_Eq = new_axiom ("prSum_Eq",
+                               ``∀P P'. P = P' ⇔ prSum P = prSum P'``);
+
+val prSum_prSumRev = new_axiom ("prSum_prSumRev",
+                          ``∀P P'. (P = (prSum P')) ⇔ ((prSumRev P) = P')``);
+                          
+val prSum_Rev = new_axiom ("prSum_Rev",
+                           ``∀P. (prSum (prSumRev P)) = P``);
+
+val Rev_prSum = new_axiom ("Rev_prSum",
+                          ``∀P. (prSumRev (prSum P)) = P``);
+                          
 val binterl_Empty = new_axiom ("binterl_Empty",
                                ``∀t1 t2. binterl t1 t2 [] ⇒ ((t1 = []) ∧(t2 = []))``);
 
+val binterl_Conj = new_axiom ("binterl_Conj",
+                              ``∀h1 t1 h2 t2 h t. (binterl ((h1::t1):('event1 + 'eventS) option list) ((h2::t2):('event2 + 'eventS) option list) (h::t)) ⇒ ((binterl t1 t2 t) ∧ (binterl [h1] [h2] [h]))``);
+
+val binterl_NotEmpty = new_axiom ("binterl_NotEmpty",
+                                  ``∀t1 t2. binterl t1 t2 (h::t) ⇒ (∃h1 t1' h2 t2'. (t1 = (h1::t1'))∧(t2 = (h2::t2')))``);
+
 val binterl_EmptyRev = new_axiom ("binterl_EmptyRev",
-                               ``∀t. binterl [] [] t ⇒ (t = [])``);
+                                  ``∀t. binterl [] [] t ⇒ (t = [])``);
                                
 val binterl_moveNONE = new_axiom ("binterl_moveNONE",
                                 ``∀e t t1 t2.
@@ -79,13 +156,53 @@ val binterl_moveAL = new_axiom ("binterl_moveAL",
 val binterl_moveAR = new_axiom ("binterl_moveAR",
                                ``∀e2 t t1 t2.
                                      binterl t1 t2 (SOME (INR (INL e2))::t) ⇒
-                                  (∃t2'. (t2 = SOME (INL e2)::t2'))``);                                  
+                                  (∃t2'. (t2 = SOME (INL e2)::t2'))``);
+
+
+ val binterl_moveNAL = new_axiom ("binterl_moveNAL",
+                               ``∀e1 t t1 t2.
+                                     binterl t1 t2 (SOME (INL (INL e1))::t) ⇒
+                                  (∃t1' t2'. (t1 = SOME (INL e1)::t1') ∧ (t2 = NONE::t2'))``);
+
+val binterl_moveNAR = new_axiom ("binterl_moveNAR",
+                                 ``∀e2 t t1 t2.
+                                       binterl t1 t2 (SOME (INR (INL e2))::t) ⇒
+                                    (∃t1' t2'. (t2 = SOME (INL e2)::t2') ∧ (t1 = NONE::t1'))``);
+
+
+val binterl_moveALN = new_axiom ("binterl_moveALN",
+                               ``∀e1.
+                                     binterl [SOME (INL e1)] [NONE] [SOME (INL (INL e1))] =
+                                  (binterl [] [] [])``);
+
+val binterl_moveSLN = new_axiom ("binterl_moveSLN",
+                               ``∀e2.
+                                     binterl [NONE] [SOME (INR e2)] [SOME (INL (INR e2))] =
+                                  (binterl [] [] [])``);
+
+val binterl_moveSRN = new_axiom ("binterl_moveSRN",
+                                 ``∀e2.                                  
+                                      binterl [NONE] [SOME (INR e2)] [SOME (INR (INR e2))] =
+                                    (binterl [] [] [])``);
+
+val binterl_moveARN = new_axiom ("binterl_moveARN",
+                               ``∀e2.
+binterl [NONE] [SOME (INL e2)] [SOME (INR (INL e2))] =
+                                  (binterl [] [] [])``); 
  
-        
+val OUTR_INL_FUN_thm = new_axiom("OUTR_INL_FUN", ``         
+∀x n.
+ OUTR (INL x) = n x``);
+
+val OUTL_INR_FUN_thm = new_axiom("OUTL_INR_FUN", ``      
+∀x n.
+ OUTL (INR x) = n x``);
+
 val TranRelNil = new_axiom ("TranRelNil",
                             ``∀(MTrn:('event, 'pred, 'state , 'symb ) mtrel) v p s. MTrn (v,p,s) [] (v,p,s)``);
 val TranRelConfigEq = new_axiom ("TranRelConfigEq",
-                            ``∀(MTrn:('event, 'pred, 'state , 'symb ) mtrel) v p s v' p' s'. (MTrn (v,p,s) [] (v',p',s')) ⇒ ((v = v')∧(p = p')∧(s = s'))``);
+                                 ``∀(MTrn:('event, 'pred, 'state , 'symb ) mtrel) v p s v' p' s'. (MTrn (v,p,s) [] (v',p',s')) ⇒ ((v = v')∧(p = p')∧(s = s'))``);
+
 val TranRelSnoc = new_axiom ("TranRelSnoc",
                              ``∀(MTrn:('event, 'pred, 'state , 'symb ) mtrel) v p s v' p' s' v'' p'' s'' t e. ((MTrn (v,p,s) t (v',p',s')) ∧ (MTrn (v',p',s') [e] (v'',p'',s''))) ⇒ (MTrn (v,p,s) (e::t) (v'',p'',s''))``);
 
@@ -97,7 +214,33 @@ val TranRelSnocRev = new_axiom ("TranRelSnocRev",
                                  
 val IMAGEOUT = new_axiom ("IMAGEOUT",
                           ``∀P P'. ((IMAGE OUTR P = IMAGE OUTR P') ∧ (IMAGE OUTL P = IMAGE OUTL P')) ⇒ (P = P')``);
-                              
+
+val combineAllDedRev21 = new_axiom ("combineAllDedRev21",
+                          ``∀(ded1:('pred1) tded) (ded2:('pred2) tded) (ded3:('pred1 + 'pred2) tded) P phi (m: 'pred2 -> 'pred1) (n: 'pred1 -> 'pred2).
+                                                  combineAllDed ded2 ded1 (RevDed ded3) P (SUM_MAP n m phi) = combineAllDed ded1 ded2 ded3 (IMAGE (SUM_MAP m n) P) phi``);
+
+val combineAllDedRev12 = new_axiom ("combineAllDedRev12",
+                          ``∀(ded1:('pred1) tded) (ded2:('pred2) tded) (ded3:('pred1 + 'pred2) tded) P phi (m: 'pred2 -> 'pred1) (n: 'pred1 -> 'pred2).
+                                                  combineAllDed ded1 ded2 ded3 P ((SUM_MAP m n) phi) = combineAllDed ded2 ded1 (RevDed ded3) (IMAGE (SUM_MAP n m) P) phi``);
+                                                  
+val combineAllDedprSum12 = new_axiom ("combineAllDedprSum12",
+                          ``∀phi ded12 ded3 comded3 P'' P' ded1 ded23 comded1.
+          (combineAllDed ded12 ded3 comded3 P'' phi ∧
+          P' = P'' ∪ {phi})
+⇒
+        (∀phi.
+          combineAllDed ded1 ded23 comded1 (prSum P'')
+            phi ∧ prSum P' = prSum P'' ∪ {phi})``);
+
+val combineAllDedprSum23 = new_axiom ("combineAllDedprSum23",
+                          ``∀phi ded12 ded3 comded3 P'' P' ded1 ded23 comded1.
+          ( combineAllDed ded1 ded23 comded1 P'' phi ∧
+          prSum P' = P'' ∪ {phi})
+⇒
+        (∀phi.
+          combineAllDed ded12 ded3 comded3 (prSumRev P'')
+            phi ∧ P' = prSumRev P'' ∪ {phi})``);
+                        
 val DedRelINL = new_axiom ("DedRelINL",
                           ``∀(ded1:('pred1) tded) (MTrn1:('event1 + 'eventS, 'pred1, 'state1, 'symb) mtrel) (MTrn2:('event2 + 'eventS, 'pred2, 'state2, 'symb) mtrel) (ded3:('pred1 + 'pred2) tded) Sym P S1 S2 Sym' P' S1' S2' P'' t1 t2 x.
                             ((MTrn1 (Sym',IMAGE OUTL P'',S1') [NONE] (Sym',IMAGE OUTL P'' ∪ {x},S1')) ∧
