HolBA/src/tools/parallelcomposition/instantiations/bir_comp_attacker_vs_sbir_comp_DYScript.sml
@@ -4,16 +4,19 @@ open pred_setTheory;
 open sigma_algebraTheory;
 open listTheory;
 open tautLib;
-open interleavingdeductionTheory;
-open parallelcompositiondeductionTheory;
+open interleavinggeneraldeductionTheory;
+open parallelcompositiongeneraldeductionTheory;
 open translate_to_sapicTheory;
-open derived_rules_deductionTheory;
+open derived_rules_generaldeductionTheory;
 open sbir_treeTheory;
 open sapicplusTheory;
 open messagesTheory;
 open dolevyaoTheory;
+open combined_deductionTheory;
 open arm8_vs_bir_comp_attackerTheory;
-open traceinclusionTheory;
+open refinementTheory;
+open parallelcompositionconcreteTheory;
+open interleavingconcreteTheory;
 open WinitexampleTheory;
 val _ = new_theory "bir_comp_attacker_vs_sbir_comp_DY";
 
@@ -33,14 +36,14 @@ val att_traces_def = Define `
 `;
     
 val sbir_traces_thm =
-INST_TYPE [``:'symb`` |-> ``:Var_t``,``:'pred`` |-> ``:'SPpred``,``:'state`` |-> ``:(sbir_event, real,(bir_var_t, bir_exp_t) symb_interpret_t) stree``,``:'event`` |-> ``:(sbir_event + (Name_t, Var_t) sync_event)``] derived_rules_deductionTheory.traces_def;
+INST_TYPE [``:'symb`` |-> ``:Var_t``,``:'pred`` |-> ``:bir_exp_t``,``:'state`` |-> ``:(sbir_event, real,(bir_var_t, bir_exp_t) symb_interpret_t) stree``,``:'event`` |-> ``:(sbir_event + (Name_t, Sig_t, Var_t) sync_event)``] derived_rules_generaldeductionTheory.traces_def;
 val sbir_traces_t = (fst o strip_comb o fst o dest_eq o snd o strip_forall o concl) sbir_traces_thm;
 val sbir_traces_def = Define `
     sbir_traces = ^(sbir_traces_t)
 `;
     
 val DY_traces_thm =
-INST_TYPE [``:'symb`` |-> ``:Var_t``,``:'pred`` |-> ``:DYpred``,``:'state`` |-> ``:DYstate``,``:'event`` |-> ``:(DYnsyc_event + (Name_t, Var_t) sync_event)``] derived_rules_deductionTheory.traces_def;
+INST_TYPE [``:'symb`` |-> ``:Var_t``,``:'pred`` |-> ``:DYpred``,``:'state`` |-> ``:DYstate``,``:'event`` |-> ``:(DYnsyc_event + (Name_t, Sig_t, Var_t) sync_event)``] derived_rules_generaldeductionTheory.traces_def;
 val DY_traces_t = (fst o strip_comb o fst o dest_eq o snd o strip_forall o concl) DY_traces_thm;
 val DY_traces_def = Define `
     DY_traces = ^(DY_traces_t)
@@ -54,7 +57,7 @@ val bir_att_comptraces_def = Define `
 `;
 
 val sbir_DY_comptraces_thm =
-INST_TYPE [``:'symb`` |-> ``:Var_t``,``:'pred1`` |-> ``:'SPpred``,``:'state1`` |-> ``:(sbir_event, real,(bir_var_t, bir_exp_t) symb_interpret_t) stree``,``:'event1`` |-> ``:sbir_event``,``:'pred2`` |-> ``:DYpred``,``:'state2`` |-> ``:DYstate``,``:'event2`` |-> ``:DYnsyc_event``,``:'eventS`` |-> ``:(Name_t, Var_t) sync_event``] derived_rules_deductionTheory.comptraces_def;
+INST_TYPE [``:'symb`` |-> ``:Var_t``,``:'pred1`` |-> ``:bir_exp_t``,``:'state1`` |-> ``:(sbir_event, real,(bir_var_t, bir_exp_t) symb_interpret_t) stree``,``:'event1`` |-> ``:sbir_event``,``:'pred2`` |-> ``:DYpred``,``:'state2`` |-> ``:DYstate``,``:'event2`` |-> ``:DYnsyc_event``,``:'eventS`` |-> ``:(Name_t, Sig_t, Var_t) sync_event``] derived_rules_generaldeductionTheory.comptraces_def;
 val sbir_DY_comptraces_t = (fst o strip_comb o fst o dest_eq o snd o strip_forall o concl) sbir_DY_comptraces_thm;
 val sbir_DY_comptraces_def = Define `
     sbir_DY_comptraces = ^(sbir_DY_comptraces_t)
@@ -64,9 +67,10 @@ val sbir_DY_comptraces_def = Define `
 val compose_bir_attacker_vs_sbir_DY_thm = store_thm(
   "compose_bir_attacker_vs_sbir_DY_thm",
   ``
-  ∀(Sym:(Var_t -> bool)) (Sym':(Var_t -> bool)) (P:('SPpred + DYpred -> bool)) (P':('SPpred + DYpred -> bool)) (T0:(sbir_event, real,(bir_var_t, bir_exp_t) symb_interpret_t) stree) (Tre:(sbir_event, real,(bir_var_t, bir_exp_t) symb_interpret_t) stree) (birprog:'observation_type bir_program_t) (AMTrn:('attevent + 'ceventS, 'cstate) mctrel) (sbir_Ded:('SPpred) tded).
+  ∀(Sym:(Var_t -> bool)) (Sym':(Var_t -> bool)) (P:(bir_exp_t + DYpred -> bool)) (P':(bir_exp_t + DYpred -> bool)) (T0:(sbir_event, real,(bir_var_t, bir_exp_t) symb_interpret_t) stree) (Tre:(sbir_event, real,(bir_var_t, bir_exp_t) symb_interpret_t) stree) (birprog:'observation_type bir_program_t) (AMTrn:('attevent + 'ceventS, 'cstate) mctrel) (sbir_Ded:(bir_exp_t) tded).
 
-        (
+    (
+    (TransEnable composeDedOverApprox (symbolic_tree_multi_transitions_with_symb,sbir_Ded) (DYmultranrel,DYdeduction)) /\
      (subset_one
       (bir_traces (((bir_mrel (birprog:'observation_type bir_program_t)): bir_state_t -> ('cevent + 'ceventS) list -> bir_state_t -> bool)) ((InterpretStOne:(sbir_event, real,(bir_var_t, bir_exp_t) symb_interpret_t) stree -> bir_state_t) T0) ((InterpretStOne:(sbir_event, real,(bir_var_t, bir_exp_t) symb_interpret_t) stree -> bir_state_t) Tre))
       (sbir_traces (symbolic_tree_multi_transitions_with_symb,sbir_Ded) (Sym,(IMAGE OUTL P),T0) (Sym',(IMAGE OUTL P'),Tre))) ∧
@@ -76,19 +80,27 @@ val compose_bir_attacker_vs_sbir_DY_thm = store_thm(
 ) ==>
 (subset_comp
    (bir_att_comptraces (composeMuRe (((bir_mrel (birprog:'observation_type bir_program_t)): bir_state_t -> ('cevent + 'ceventS) list -> bir_state_t -> bool)) AMTrn) (((InterpretStOne:(sbir_event, real,(bir_var_t, bir_exp_t) symb_interpret_t) stree -> bir_state_t) T0),((InterpretStTwo:DYstate -> 'cstate) ESt)) (((InterpretStOne:(sbir_event, real,(bir_var_t, bir_exp_t) symb_interpret_t) stree -> bir_state_t) Tre),((InterpretStTwo:DYstate -> 'cstate) ESt)))
-   (sbir_DY_comptraces (symbolic_tree_multi_transitions_with_symb,sbir_Ded) (DYmultranrel,DYdeduction) (Sym,P,T0,ESt) (Sym',P',Tre,ESt))
+   (sbir_DY_comptraces (symbolic_tree_multi_transitions_with_symb,sbir_Ded) (DYmultranrel,DYdeduction) composeDedOverApprox (Sym,P,T0,ESt) (Sym',P',Tre,ESt))
 )
-``,
-rewrite_tac[interleavingconcreteTheory.binterleave_composition_concrete,binterleave_composition_deduction,interleavingconcreteTheory.binterleave_ts,interleavingdeductionTheory.binterleave_ts,derived_rules_deductionTheory.traces_def,interleavingconcreteTheory.traces_def,sbir_DY_comptraces_def,bir_att_comptraces_def,DY_traces_def,sbir_traces_def,att_traces_def,bir_traces_def]>>
-  FULL_SIMP_TAC (list_ss++pred_setSimps.PRED_SET_ss++boolSimps.LIFT_COND_ss++boolSimps.EQUIV_EXTRACT_ss) [subset_one_def,subset_two_def,subset_comp_def]>>
-  rw[] >>
-  PAT_X_ASSUM ``!x. A`` (ASSUME_TAC o (Q.SPECL [`((RevInterpretEvTwoSyn:('attevent + 'ceventS) list -> (DYnsyc_event + (Name_t, Var_t) sync_event) option list) (t2:(('attevent+'ceventS) list)))`]))>>
-  PAT_X_ASSUM ``!x. A`` (ASSUME_TAC o (Q.SPECL [`((RevInterpretEvOneSyn:('cevent + 'ceventS) list -> (sbir_event + (Name_t, Var_t) sync_event) option list) (t1:(('cevent + 'ceventS) list)))`]))>>
-  FULL_SIMP_TAC (list_ss++pred_setSimps.PRED_SET_ss++boolSimps.LIFT_COND_ss++boolSimps.EQUIV_EXTRACT_ss) [applyfunEvOneSyn,applyfunEvTwoSyn]>>            
-  RES_TAC>>
-  Q.EXISTS_TAC `((RevInterpretEvOneSyn:('cevent + 'ceventS) list -> (sbir_event + (Name_t, Var_t) sync_event) option list) t1)` >>
-  Q.EXISTS_TAC `((RevInterpretEvTwoSyn:('attevent + 'ceventS) list -> (DYnsyc_event + (Name_t, Var_t) sync_event) option list) t2)` >>
-  metis_tac[binterl_Rev]
+``, 
+  
+rewrite_tac[sbir_DY_comptraces_def,bir_att_comptraces_def,DY_traces_def,sbir_traces_def,att_traces_def,bir_traces_def,binterleave_composition_concrete,interleavingconcreteTheory.binterleave_ts,interleavinggeneraldeductionTheory.binterleave_ts,derived_rules_generaldeductionTheory.traces_def,interleavingconcreteTheory.traces_def]>>
+FULL_SIMP_TAC (list_ss++pred_setSimps.PRED_SET_ss++boolSimps.LIFT_COND_ss++boolSimps.EQUIV_EXTRACT_ss) [subset_one_def,subset_two_def,subset_comp_def]>>
+  rw[]>>
+ Q.EXISTS_TAC `InterpretEvComp` >>
+rw[] >>
+PAT_X_ASSUM ``!x. A`` (ASSUME_TAC o (Q.SPECL [`((RevInterpretEvTwoSyn:('attevent + 'ceventS) list -> (DYnsyc_event + (Name_t, Sig_t, Var_t) sync_event) option list) (t2:(('attevent+'ceventS) list)))`]))>>
+  PAT_X_ASSUM ``!x. A`` (ASSUME_TAC o (Q.SPECL [`((RevInterpretEvOneSyn:('cevent + 'ceventS) list -> (sbir_event + (Name_t, Sig_t, Var_t) sync_event) option list) (t1:(('cevent + 'ceventS) list)))`]))>>
+FULL_SIMP_TAC (list_ss++pred_setSimps.PRED_SET_ss++boolSimps.LIFT_COND_ss++boolSimps.EQUIV_EXTRACT_ss) [applyfunEvOneSyn,applyfunEvTwoSyn]>>            
+RES_TAC>>
+IMP_RES_TAC binterleave_composition_generaldeduction_supseteq >>
+PAT_X_ASSUM ``!Sym' Sym S2' S2 S1' S1 P' P. A`` (ASSUME_TAC o (Q.SPECL [`Sym'`,`Sym`,`ESt`,`ESt`,`Tre`,`T0`,`P'`,`P`])) >>
+RES_TAC >>
+FULL_SIMP_TAC (list_ss++pred_setSimps.PRED_SET_ss++boolSimps.LIFT_COND_ss++boolSimps.EQUIV_EXTRACT_ss) [SUBSET_DEF] >>
+PAT_X_ASSUM ``!x. A`` (ASSUME_TAC o (Q.SPECL [`x`])) >>
+FULL_SIMP_TAC (list_ss++pred_setSimps.PRED_SET_ss++boolSimps.LIFT_COND_ss++boolSimps.EQUIV_EXTRACT_ss) [interleavinggeneraldeductionTheory.binterleave_ts,derived_rules_generaldeductionTheory.traces_def,derived_rules_generaldeductionTheory.comptraces_def] >>
+IMP_RES_TAC binterl_Rev >>
+RES_TAC
 );
 
         
@@ -97,13 +109,13 @@ val birprog_def = Define `
     birprog = ^(birprog_t)
 `;
 
-       
+     
 val compose_birexample_attacker_vs_sbir_DY_thm = store_thm(
   "compose_birexample_attacker_vs_sbir_DY_thm",
   ``
-  ∀(Sym:(Var_t -> bool)) (Sym':(Var_t -> bool)) (P:('SPpred + DYpred -> bool)) (P':('SPpred + DYpred -> bool)) (T0:(sbir_event, real,(bir_var_t, bir_exp_t) symb_interpret_t) stree) (Tre:(sbir_event, real,(bir_var_t, bir_exp_t) symb_interpret_t) stree) (AMTrn:('attevent + 'ceventS, 'cstate) mctrel) (sbir_Ded:('SPpred) tded).
+  ∀(Sym:(Var_t -> bool)) (Sym':(Var_t -> bool)) (P:(bir_exp_t + DYpred -> bool)) (P':(bir_exp_t + DYpred -> bool)) (T0:(sbir_event, real,(bir_var_t, bir_exp_t) symb_interpret_t) stree) (Tre:(sbir_event, real,(bir_var_t, bir_exp_t) symb_interpret_t) stree) (AMTrn:('attevent + 'ceventS, 'cstate) mctrel) (sbir_Ded:(bir_exp_t) tded).
 
-        (
+        ((TransEnable composeDedOverApprox (symbolic_tree_multi_transitions_with_symb,sbir_Ded) (DYmultranrel,DYdeduction)) /\
      (subset_one
       (bir_traces (((bir_mrel (birprog:'observation_type bir_program_t)): bir_state_t -> ('cevent + 'ceventS) list -> bir_state_t -> bool)) ((InterpretStOne:(sbir_event, real,(bir_var_t, bir_exp_t) symb_interpret_t) stree -> bir_state_t) T0) ((InterpretStOne:(sbir_event, real,(bir_var_t, bir_exp_t) symb_interpret_t) stree -> bir_state_t) Tre))
       (sbir_traces (symbolic_tree_multi_transitions_with_symb,sbir_Ded) (Sym,(IMAGE OUTL P),T0) (Sym',(IMAGE OUTL P'),Tre))) ∧
@@ -113,7 +125,7 @@ val compose_birexample_attacker_vs_sbir_DY_thm = store_thm(
 ) ==>
 (subset_comp
    (bir_att_comptraces (composeMuRe (((bir_mrel (birprog:'observation_type bir_program_t)): bir_state_t -> ('cevent + 'ceventS) list -> bir_state_t -> bool)) AMTrn) (((InterpretStOne:(sbir_event, real,(bir_var_t, bir_exp_t) symb_interpret_t) stree -> bir_state_t) T0),((InterpretStTwo:DYstate -> 'cstate) ESt)) (((InterpretStOne:(sbir_event, real,(bir_var_t, bir_exp_t) symb_interpret_t) stree -> bir_state_t) Tre),((InterpretStTwo:DYstate -> 'cstate) ESt)))
-   (sbir_DY_comptraces (symbolic_tree_multi_transitions_with_symb,sbir_Ded) (DYmultranrel,DYdeduction) (Sym,P,T0,ESt) (Sym',P',Tre,ESt))
+   (sbir_DY_comptraces (symbolic_tree_multi_transitions_with_symb,sbir_Ded) (DYmultranrel,DYdeduction) composeDedOverApprox (Sym,P,T0,ESt) (Sym',P',Tre,ESt))
 )
 ``,
 metis_tac[compose_bir_attacker_vs_sbir_DY_thm]
