HolBA/src/tools/parallelcomposition/sapic/dolevyaoScript.sml
@@ -1,35 +1,51 @@
 open HolKernel Parse boolLib bossLib;
 open messagesTheory;
 open synceventsTheory;
+open listTheory;
 
 val _ = new_theory "dolevyao";
 
-    
+
 (* Dolev-Yao predicates *)
 val _ = Datatype `DYpred =
 K SapicTerm_t (* Adversary can deduce term *)
 | Fr SapicTerm_t (* Term is fresh *)
-| Equ (SapicTerm_t # SapicTerm_t) (* both terms *)
+| DotEqu (SapicTerm_t # SapicTerm_t) (* both terms *)
+| AliEqu (Var_t # SapicTerm_t) (* both terms *)
       `;
     
+(* val _ = Theory.new_constant("eqE", ``:SapicTerm_t -> SapicTerm_t -> bool``); *)
 
-      
+
+Inductive eqE:
+[~ref:]
+  (∀(t:SapicTerm_t). (eqE t t)) /\
+[~sym:]
+(∀(t1:SapicTerm_t) (t2:SapicTerm_t). (eqE t1 t2) ==> (eqE t2 t1)) /\
+[~tran:]
+(∀(t1:SapicTerm_t) (t2:SapicTerm_t) (t3:SapicTerm_t). ((eqE t1 t2)  /\ (eqE t2 t3) )==> (eqE t1 t3)) 
+End        
+    
+val eqE_not = new_axiom ("eqE_not",
+                               ``(∀(t1:SapicTerm_t) (t2:SapicTerm_t). (t1 ≠ t2) ==> (¬(eqE t1 t2)))``);
+
 (* Dolev-Yao deduction relation *)
 val (DYdeduction_rules, DYdeduction_ind, DYdeduction_cases)
 = Hol_reln
   `(∀(p:DYpred) (Pi: DYpred set). (p ∈ Pi) ==> (DYdeduction Pi p)) ∧
   (∀(n:SapicTerm_t) (Pi: DYpred set). (n = (Con (Name (PubName:NameTag_t) (str:string)))) ==> (DYdeduction Pi (K n))) ∧
-(∀(k:SapicTerm_t) (m:SapicTerm_t) (Pi: DYpred set). ((DYdeduction Pi (K k)) ∧ (DYdeduction Pi (K m))) ==> (DYdeduction Pi (K (FAPP  ("Enc", (2, Public, Constructor)) [m;k])))) ∧
-(∀(k:SapicTerm_t) (m:SapicTerm_t) (Pi: DYpred set). ((DYdeduction Pi (K k)) ∧ (DYdeduction Pi (K (FAPP  ("Enc", (2, Public, Constructor)) [m;k])))) ==> (DYdeduction Pi (K m))) ∧
-(∀(t1:SapicTerm_t) (t2:SapicTerm_t) (Pi: DYpred set). ((DYdeduction Pi (K t1)) ∧ (DYdeduction Pi (Equ (t1,t2)))) ==> (DYdeduction Pi (K t2))) ∧
-(∀(n1:SapicTerm_t) (n2:SapicTerm_t) (Pi: DYpred set). ((DYdeduction Pi (Fr n1)) ∧ (DYdeduction Pi (Equ (n1,n2)))) ==> (DYdeduction Pi (Fr n2))) 
+(∀(sig:(string # (int # Privacy_t # Constructability_t))) (tl:SapicTerm_t list) (Pi: DYpred set). (EVERY (DYdeduction Pi) (MAP K tl)) ==> (DYdeduction Pi (K (FAPP sig tl)))) ∧
+(∀(t1:SapicTerm_t) (t2:SapicTerm_t) (Pi: DYpred set). ((DYdeduction Pi (K t1)) ∧ (DYdeduction Pi (DotEqu (t1,t2)))) ==> (DYdeduction Pi (K t2))) ∧
+(∀(n1:SapicTerm_t) (n2:SapicTerm_t) (Pi: DYpred set). ((DYdeduction Pi (Fr n1)) ∧ (DYdeduction Pi (DotEqu (n1,n2)))) ==> (DYdeduction Pi (Fr n2))) ∧
+(∀(t1:SapicTerm_t) (t2:SapicTerm_t) (v:Var_t) (Pi: DYpred set). ((DYdeduction Pi (K t1)) ∧ (DYdeduction Pi (AliEqu (v,t2)))) ==> (DYdeduction Pi (K (sapic_substvar v t2 t1)))) ∧
+(∀(t1:SapicTerm_t) (t2:SapicTerm_t) (Pi: DYpred set). (eqE t1 t2) ==> (DYdeduction Pi (DotEqu (t1,t2)))) 
 `;
-
 
 (* Dolev-Yao non-synchronous events *)        
 val _ = Datatype
         `DYnsyc_event =
 Silent Name_t
+| Ded DYpred
 | Alias (Var_t # SapicTerm_t)
         `;
 
@@ -45,10 +61,12 @@ ESt       (* empty state *)
 val DYtranrel_def =
 Define` 
       (DYtranrel (Sym,Pi,ESt) (SOME (INR (P2A Y))) (Sym',Pi',ESt) = ((Y ∉ Sym) ∧ (Pi' = Pi∪{K (TVar Y)}) ∧ (Sym = Sym'))) ∧
-      (DYtranrel (Sym,Pi,ESt) (SOME (INL (Alias (X',Y')))) (Sym',Pi',ESt) = ((X' ∉ Sym) ∧ (Sym' = Sym∪{X'}) ∧ (Pi' = Pi∪{Equ((TVar X'),Y')}))) ∧
+      (DYtranrel (Sym,Pi,ESt) (SOME (INL (Alias (X',Y')))) (Sym',Pi',ESt) = ((X' ∉ Sym) ∧ (Sym' = Sym∪{X'}) ∧ (Pi' = Pi∪{AliEqu(X',Y')}))) ∧
+      (DYtranrel (Sym,Pi,ESt) (SOME (INR (Crypto (S,XL,Y)))) (Sym',Pi',ESt) = ((EVERY Sym XL) ∧ (Y ∉ Sym) ∧ (Sym' = Sym∪{Y}) ∧ (Pi' = Pi∪{AliEqu(Y,(FAPP S (MAP TVar XL)))}))) ∧
       (DYtranrel (Sym,Pi,ESt) (SOME (INR (A2P X))) (Sym',Pi',ESt) = ((K (TVar X) ∈ Pi) ∧ (Pi = Pi') ∧ (Sym = Sym'))) ∧
       (DYtranrel (Sym,Pi,ESt) (SOME (INL (Silent n))) (Sym',Pi',ESt) = ((Fr (Con n) ∉ Pi ) ∧ (Pi' = Pi∪{(Fr (Con n));(K (Con n))}) ∧ (Sym = Sym'))) ∧
       (DYtranrel (Sym,Pi,ESt) (SOME (INR (Sync_Fr n'))) (Sym',Pi',ESt) = ((Fr (Con n') ∉ Pi ) ∧ (Pi' = Pi∪{Fr (Con n')}) ∧ (Sym = Sym'))) ∧
+      (DYtranrel (Sym,Pi,ESt) (SOME (INL (Ded p))) (Sym',Pi',ESt) = ((Pi' = Pi∪{p}) ∧ (DYdeduction Pi p) ∧ (Sym = Sym'))) ∧
       (DYtranrel (Sym,Pi,ESt) (NONE) (Sym',Pi',ESt) = ((Pi = Pi') ∧ (Sym = Sym')))
 `;                                      
 
@@ -56,18 +74,18 @@ Define`
 (* Dolev-Yao multi transition relation *)
 Inductive DYmultranrel:
 [~nil:]
-  (DYmultranrel ((Sym:(Var_t -> bool)),(P:(DYpred -> bool)),ESt) ([]:(DYnsyc_event + (Name_t,Var_t) sync_event) option list) ((Sym:(Var_t -> bool)),(P:(DYpred -> bool)),ESt)) /\
+  (DYmultranrel ((Sym:(Var_t -> bool)),(P:(DYpred -> bool)),ESt) ([]:(DYnsyc_event + (Name_t,Sig_t,Var_t) sync_event) option list) ((Sym:(Var_t -> bool)),(P:(DYpred -> bool)),ESt)) /\
 [~move:]
   (
-  ((DYmultranrel ((Sym:(Var_t -> bool)),(P:(DYpred -> bool)),ESt) (ev:(DYnsyc_event + (Name_t,Var_t) sync_event) option list) ((Sym'':(Var_t -> bool)),(P'':(DYpred -> bool)),ESt)) /\
-   (DYtranrel ((Sym'':(Var_t -> bool)),(P'':(DYpred -> bool)),ESt) (e:(DYnsyc_event + (Name_t,Var_t) sync_event) option) ((Sym':(Var_t -> bool)),(P':(DYpred -> bool)),ESt))) ==>
-  ((DYmultranrel ((Sym:(Var_t -> bool)),(P:(DYpred -> bool)),ESt) ((e::ev):(DYnsyc_event + (Name_t,Var_t) sync_event) option list) ((Sym':(Var_t -> bool)),(P':(DYpred -> bool)),ESt)))
+  ((DYmultranrel ((Sym:(Var_t -> bool)),(P:(DYpred -> bool)),ESt) (ev:(DYnsyc_event + (Name_t,Sig_t,Var_t) sync_event) option list) ((Sym'':(Var_t -> bool)),(P'':(DYpred -> bool)),ESt)) /\
+   (DYtranrel ((Sym'':(Var_t -> bool)),(P'':(DYpred -> bool)),ESt) (e:(DYnsyc_event + (Name_t,Sig_t,Var_t) sync_event) option) ((Sym':(Var_t -> bool)),(P':(DYpred -> bool)),ESt))) ==>
+  ((DYmultranrel ((Sym:(Var_t -> bool)),(P:(DYpred -> bool)),ESt) ((e::ev):(DYnsyc_event + (Name_t,Sig_t,Var_t) sync_event) option list) ((Sym':(Var_t -> bool)),(P':(DYpred -> bool)),ESt)))
   )
 End
 
 val DYmultranrel_single = new_axiom ("DYmultranrel_single",
                                      ``∀e Sym Sym' P P'.
-                                              (DYmultranrel ((Sym:(Var_t -> bool)),(P:(DYpred -> bool)),ESt) ([e]:(DYnsyc_event + (Name_t,Var_t) sync_event) option list) ((Sym':(Var_t -> bool)),(P':(DYpred -> bool)),ESt)) =
-  (DYtranrel ((Sym:(Var_t -> bool)),(P:(DYpred -> bool)),ESt) (e:(DYnsyc_event + (Name_t,Var_t) sync_event) option) ((Sym':(Var_t -> bool)),(P':(DYpred -> bool)),ESt)) ``);
+                                              (DYmultranrel ((Sym:(Var_t -> bool)),(P:(DYpred -> bool)),ESt) ([e]:(DYnsyc_event + (Name_t,Sig_t,Var_t) sync_event) option list) ((Sym':(Var_t -> bool)),(P':(DYpred -> bool)),ESt)) =
+  (DYtranrel ((Sym:(Var_t -> bool)),(P:(DYpred -> bool)),ESt) (e:(DYnsyc_event + (Name_t,Sig_t,Var_t) sync_event) option) ((Sym':(Var_t -> bool)),(P':(DYpred -> bool)),ESt)) ``);
                                                  
 val _ = export_theory();
