HolBA/src/tools/parallelcomposition/sapic/synceventsScript.sml
@@ -7,7 +7,8 @@ val _ = new_theory "syncevents";
 
 val _ = Datatype `sync_event =
     P2A 'v
-    | A2P 'v
+| A2P 'v
+| Crypto ('s # 'v list # 'v)
     | Sync_Fr 'n
                 `;
                 
